Swithcing to base graph data structures on sets rather than functions.  Everything broken.

Circuit/CircuitBase.dfy
@@ -28,15 +28,31 @@ module CircuitBase {
         )
 
     datatype Circuit = Circuit(
-        NodeKind: CNode -> Option<CNodeKind>,
-        PortSource: NP -> Option<NP>,
+        NodeKind: map<CNode, CNodeKind>,//CNode -> Option<CNodeKind>,
+        PortSource: map<NP, NP>,
         // This is larger or equal to all nodes for which NodeKind(node) is Some
         // We use this help dafny prove that things are finite and terminate.
-        NodeBound: CNode,
-        PortBound: CPort,
+        //NodeBound: CNode,
+        //PortBound: CPort,
         HierLevel: nat,
-        PortNames: string -> Option<CNode>
+        PortNames: map<string, CNode>
     )
+
+    function NodeKind(c: Circuit, n: CNode): Option<CNodeKind>
+    {
+        if n in c.NodeKind then
+            Some(c.NodeKind[n])
+        else
+            None
+    }
+
+    function PortSource(c: Circuit, np: NP): Option<NP>
+    {
+        if np in c.PortSource then
+            Some(c.PortSource[np])
+        else
+            None
+    }
 
     datatype CNodeKind = 
         // A hierarchical node so we can design hierarchically.
@@ -64,12 +80,37 @@ module CircuitBase {
         // The port numbers of a hierarical block and just the node ids of
         // the input and output nodes.
         case CHier(subc) =>
-            set n | n < subc.NodeBound && subc.NodeKind(n) == Some(CInput) :: n as CPort
+            set n | n in subc.NodeKind && subc.NodeKind[n] == CInput :: n as CPort
         case CComb(iports, oports, path_exists, behav, names) => Seq.ToSet(iports)
         case CInput() => {}
         case CConst(v) => {}
-        case COutput() => {0 as CPort}
-        case CSeq() => {0 as CPort}
+        case COutput() => {INPUT_PORT as CPort}
+        case CSeq() => {INPUT_PORT as CPort}
+    }
+
+    predicate IsPort(nk: CNodeKind, p: CPort)
+    {
+        IsIPort(nk, p) || IsOPort(nk, p)
+    }
+
+    lemma InIPortsIsIPort(nk: CNodeKind, p: CPort)
+        requires IsIPort(nk, p)
+        ensures p in IPorts(nk)
+    {
+        reveal Seq.ToSet();
+    }
+    lemma InOPortsIsOPort(nk: CNodeKind, p: CPort)
+        requires IsOPort(nk, p)
+        ensures p in OPorts(nk)
+    {
+        reveal Seq.ToSet();
+        match nk
+        case CHier(subc) => {}
+        case CComb(iports, oports, path_exists, behav, name) => {}
+        case CInput() => {}
+        case CConst(v) => {}
+        case COutput() => {}
+        case CSeq() => {}
     }
 
     predicate IsIPort(nk: CNodeKind, p: CPort)
@@ -77,7 +118,7 @@ module CircuitBase {
         match nk
         // The port numbers of a hierarical block and just the node ids of
         // the input and output nodes.
-        case CHier(subc) => subc.NodeKind(p as CNode) == Some(CInput)
+        case CHier(subc) => NodeKind(subc, p as CNode) == Some(CInput)
         case CComb(iports, oports, path_exists, behav, name) => p in iports
         case CInput() => false
         case CConst(v) => false
@@ -89,12 +130,12 @@ module CircuitBase {
     {
         match nk
         case CHier(subc) =>
-            set n | n < subc.NodeBound && subc.NodeKind(n) == Some(COutput) :: n as CPort
+            set n | n in subc.NodeKind && subc.NodeKind[n] == COutput :: n as CPort
         case CComb(iports, oports, path_exists, behav, names) => Seq.ToSet(oports)
-        case CInput() => {0 as CPort}
+        case CInput() => {OUTPUT_PORT as CPort}
         case COutput() => {}
-        case CConst(v) => {0 as CPort}
-        case CSeq() => {0 as CPort}
+        case CConst(v) => {OUTPUT_PORT as CPort}
+        case CSeq() => {OUTPUT_PORT as CPort}
     }
 
     predicate IsOPort(nk: CNodeKind, p: CPort)
@@ -103,7 +144,7 @@ module CircuitBase {
         // The port numbers of a hierarical block and just the node ids of
         // the input and output nodes.
         case CHier(subc) =>
-            subc.NodeKind(p as CNode) == Some(COutput)
+            NodeKind(subc, p as CNode) == Some(COutput)
         case CComb(iports, oports, path_exists, behav, names) => p in oports
         case CInput() => p == OUTPUT_PORT as CPort
         case CConst(v) => p == OUTPUT_PORT as CPort
@@ -126,8 +167,20 @@ module CircuitBase {
         )
     }
 
+    lemma CNodeKindNoSelfPaths(nk: CNodeKind)
+        requires CNodeKindSomewhatValid(nk)
+        requires nk.CComb?
+        ensures forall p: CPort :: !nk.PathExists(p, p)
+    {
+        forall p: CPort
+            ensures !nk.PathExists(p, p)
+        {
+            assert !(IsIPort(nk, p) && IsOPort(nk, p));
+        }
+    }
+
     ghost predicate CNodeKindValid(
-        hier_level: nat, port_bound: CPort, nk: CNodeKind)
+        hier_level: nat, nk: CNodeKind)
         decreases hier_level, 0
     {
         CNodeKindSomewhatValid(nk) &&
@@ -137,10 +190,6 @@ module CircuitBase {
             (subc.HierLevel < hier_level) &&
             CircuitValid(subc)
         case _ => true
-        ) && (
-            forall p: CPort ::
-                (IsIPort(nk, p) ==> p < port_bound) &&
-                (IsOPort(nk, p) ==> p < port_bound)
         )
     }
 
@@ -154,16 +203,12 @@ module CircuitBase {
     ghost predicate CircuitNodeKindValid(c: Circuit)
         decreases  c.HierLevel, 1
     {
-        (
-            forall n: CNode ::
-                var maybe_nk := c.NodeKind(n);
-                if maybe_nk.None? then
-                    true
-                else
-                    CNodeKindValid(c.HierLevel, c.PortBound, maybe_nk.Extract())
-        ) && (
-            forall n: CNode :: n >= c.NodeBound ==> c.NodeKind(n) == None
-        )
+        forall n: CNode ::
+            var maybe_nk := NodeKind(c, n);
+            if maybe_nk.None? then
+                true
+            else
+                CNodeKindValid(c.HierLevel, maybe_nk.Extract())
     }
 
     ghost predicate CircuitPortSourceValid(c: Circuit)
@@ -176,14 +221,14 @@ module CircuitBase {
             forall p: CPort ::
                 var inp := NP(n, p);
                 if NPValidInput(c, inp) then
-                    match c.PortSource(inp)
+                    match PortSource(c, inp)
                     // It's ok if it doesn't connect to anything.
                     // We consider that a valid circuit, but not a complete circuit.
                     // That way we can build a circuit but it is still valid.
                     case None => true
                     case Some(onp) => NPValidOutput(c, onp)
                 else
-                    c.PortSource(inp) == None
+                    PortSource(c, inp) == None
     }
 
     ghost predicate NPValid(c: Circuit, np: NP)
@@ -193,7 +238,7 @@ module CircuitBase {
 
     ghost predicate NPValidInput(c: Circuit, np: NP)
     {
-        match c.NodeKind(np.n)
+        match NodeKind(c, np.n)
         // The node doesn't exist.
         case None => false
         case Some(nk) => IsIPort(nk, np.p)
@@ -201,8 +246,24 @@ module CircuitBase {
 
     ghost predicate NPValidOutput(c: Circuit, np: NP)
     {
-        match c.NodeKind(np.n)
+        match NodeKind(c, np.n)
         case None => false
         case Some(nk) => IsOPort(nk, np.p)
     }
+
+    predicate CNodeIsCHier(c: Circuit, n: CNode)
+    {
+        NodeKind(c, n).Some? && NodeKind(c, n).value.CHier?
+    }
+
+    predicate CNodeIsCInput(c: Circuit, n: CNode)
+    {
+        NodeKind(c, n).Some? && NodeKind(c, n).value.CInput?
+    }
+
+    predicate CNodeIsCOutput(c: Circuit, n: CNode)
+    {
+        NodeKind(c, n).Some? && NodeKind(c, n).value.COutput?
+    }
+
 }
