Circuit/CircuitBuild.dfy
@@ -4,10 +4,11 @@ module CircuitBuild {
     import opened CircuitHPNP
     import opened CircuitBase
     import opened CircuitHierarchy
-    import opened CircuitPortBounds
     import opened CircuitToGraph
+    import DG = DigraphBase
     import DP = DigraphPaths
     import DSB = DigraphStepBack
+    import DC = DigraphCombine
 
     // Proove that there are no loops in a small circuit.
     // Take a set of HPNP.
@@ -75,21 +76,18 @@ module CircuitBuild {
         ensures
             var g := CtoG(c);
             DG.DigraphValid(g) &&
-            DG.NodeValid(g, n) &&
             (StepBack(c, n) == DSB.StepBack(g, n))
     {
         var g := CtoG(c);
         CtoGValid(c);
         reveal CtoG();
         assert DG.DigraphValid(g);
-        HPNPInBound(c, n);
-        assert DG.NodeValid(g, n);
         reveal HPNPConnected();
         reveal HPNPItoOConnected();
         reveal HPNPOtoIConnected();
         StepBackMatchesHPNPConnected(c, n);
-        assert forall m :: m in DSB.StepBack(g, n) ==> g.IsConnected(n, m);
-        assert forall m :: m in StepBack(c, n) ==> g.IsConnected(n, m);
+        assert forall m :: m in DSB.StepBack(g, n) ==> DG.IsConnected(g, n, m);
+        assert forall m :: m in StepBack(c, n) ==> DG.IsConnected(g, n, m);
     }
 
     lemma EmptyCircuitHasNoHP(hp: HierarchyPath)
@@ -116,7 +114,7 @@ module CircuitBuild {
         reveal HPNPValidInput();
         reveal HPNPValidOutput();
         var c := MakeEmptyCircuit();
-        assert forall n: CNode :: c.NodeKind(n) == None;
+        assert forall n: CNode :: NodeKind(c, n) == None;
         forall hpnp: HPNP
             ensures !HPNPValid(c, hpnp)
         {
@@ -152,12 +150,10 @@ module CircuitBuild {
     {
         reveal CircuitValid();
         var c := Circuit(
-            NodeKind := _ => None,
-            PortSource := _ => None,
-            NodeBound := 0,
-            PortBound := 0,
+            NodeKind := map[],
+            PortSource := map[],
             HierLevel := 0,
-            PortNames := _ => None
+            PortNames := map[]
         );
         c
     }
@@ -177,8 +173,8 @@ module CircuitBuild {
         ensures
             var c := MakeEmptyCircuit();
             var g := CtoGV(c);
-            (forall n: HPNP :: !g.IsNode(n)) &&
-            (forall n, m: HPNP :: !g.IsConnected(n, m)) &&
+            (forall n: HPNP :: !DG.IsNode(g, n)) &&
+            (forall n, m: HPNP :: !DG.IsConnected(g, n, m)) &&
             (!DP.DigraphLoop(g))
     {
         var c := MakeEmptyCircuit();
@@ -187,9 +183,9 @@ module CircuitBuild {
         reveal CtoG();
         assert DG.DigraphValid(g);
         assert forall n: HPNP :: !HPNPValid(c, n);
-        assert forall n: HPNP :: !g.IsNode(n);
+        assert forall n: HPNP :: !DG.IsNode(g, n);
         EmptyCircuitHasNoHPNPConnected();
-        assert forall n, m: HPNP :: !g.IsConnected(n, m);
+        assert forall n, m: HPNP :: !DG.IsConnected(g, n, m);
         reveal DP.DigraphLoop();
         reveal DG.PathValid();
         assert !DP.DigraphLoop(g);
@@ -211,10 +207,227 @@ module CircuitBuild {
         c
     }
 
-    //function AddNodeEquiv(c: Circuit, nk: CNodeKind, ip: map<CPort, NP>)
+    //function NodeKindElementBound(c: Circuit, nk: CNodeKind, n: CNode): nat
+    //    requires CircuitValid(c)
+    //    requires !nk.CHier?
     //{
-    //    var new_c := AddNode(c, nk, ip);
+    //    var max_index := HPNPElementBound(c);
+    //    var port_bound := NKPortBound(nk) as nat;
+    //    var new_max_index_intermed := if port_bound > max_index then port_bound else max_index;
+    //    var new_max_index := if (n as nat)+1 > new_max_index_intermed then (n as nat)+1 else new_max_index_intermed;
+    //    new_max_index
     //}
+
+    //function NodeKindBound(c: Circuit, nk: CNodeKind, n: CNode): nat
+    //    requires CircuitValid(c)
+    //    requires !nk.CHier?
+    //{
+    //    var element_bound := NodeKindElementBound(c, nk, n);
+    //    var ns := Seq.Repeat(element_bound, c.HierLevel+2);
+    //    SeqNatToNat.ArbLenNatsToNat(ns)
+    //}
+
+    //lemma NodeKindBoundBinds(c: Circuit, nk: CNodeKind, hpn: HPNode)
+    //    requires CircuitValid(c)
+    //    requires HierarchyPathValid(c, hpn.hp)
+    //    requires !nk.CHier?
+    //    ensures
+    //        var g := NodeKindToGraph(c, nk, hpn);
+    //        var bound := NodeKindBound(c, nk, hpn.n);
+    //        forall n: HPNP :: g.IsNode(n) ==> g.NodeMap(n) < bound
+    //{
+    //    var g := NodeKindToGraph(c, nk, hpn);
+    //    var bound := NodeKindBound(c, nk, hpn.n);
+    //    assert g.NodeBound == bound;
+    //    assert forall hpnp :: g.IsNode(hpnp) ==> hpnp.hpn == hpn;
+
+    //    var element_bound := NodeKindElementBound(c, nk, hpn.n);
+    //    var ns := Seq.Repeat(element_bound, c.HierLevel+2);
+    //    assert bound == SeqNatToNat.ArbLenNatsToNat(ns);
+
+    //    HPElementsInBound(c, hpn.hp);
+    //    assert forall n: CNode :: (n in hpn.hp.v) ==> n as nat < element_bound;
+    //    assert forall e: nat :: e in SeqCNodeToSeqNat(hpn.hp.v) ==> e < element_bound;
+    //    assert hpn.n as nat < element_bound;
+
+    //    forall hpnp | g.IsNode(hpnp)
+    //        ensures HPNPToNat(hpnp) < bound
+    //    {
+    //        assert hpnp.hpn == hpn;
+    //        var hpnp_as_seqnat := HPNPToSeqNat(hpnp);
+    //        assert |hpnp_as_seqnat| == |hpnp.hpn.hp.v| + 2;
+    //        HPLengthBound(c, hpnp.hpn.hp);
+    //        assert |hpnp.hpn.hp.v| <= c.HierLevel;
+    //        assert |hpnp_as_seqnat| <= c.HierLevel + 2;
+    //        assert hpnp.p as nat < element_bound;
+    //        var as_nat := HPNPToSeqNat(hpnp);
+    //        assert forall n: nat :: n in as_nat ==> n < element_bound;
+    //        SeqNatToNat.ArbLenNatsToNatBounded(as_nat, c.HierLevel+2, element_bound);
+    //        assert HPNPToNat(hpnp) < bound;
+    //    }
+    //}
+
+    lemma {:vcs_split_on_every_assert} NodeKindToGraphNoLoop(c: Circuit, nk: CNodeKind, hpn: HPNode)
+        requires CircuitValid(c)
+        requires CNodeKindSomewhatValid(nk)
+        requires HierarchyPathValid(c, hpn.hp)
+        requires !nk.CHier?
+        ensures !DP.DigraphLoop(NodeKindToGraph(c, nk, hpn))
+    {
+        var g := NodeKindToGraph(c, nk, hpn);
+        if nk.CComb? {
+            forall p: DG.Path<HPNP> | DG.PathValid(g, p)
+                ensures !DP.PathLoop(p)
+            {
+                reveal DG.PathValid();
+                if |p.v| > 2 {
+                    assert DG.IsConnected(g, p.v[0], p.v[1]);
+                    assert p.v[0].p in nk.OPorts;
+                    assert p.v[1].p in nk.IPorts;
+                    assert p.v[1].p !in nk.OPorts;
+                    assert DG.IsConnected(g, p.v[1], p.v[2]);
+                    assert false;
+                } else if |p.v| == 2 {
+                    assert p.v[0] != p.v[1];
+                    assert !DP.PathLoop(p);
+                } else {
+                    assert !DP.PathLoop(p);
+                }
+            }
+            assert !exists p: DG.Path<HPNP> :: DG.PathValid(g, p) && DP.PathLoop(p);
+            reveal DP.DigraphLoop();
+            assert !DP.DigraphLoop(g);
+        } else {
+            assert forall n, m: HPNP :: !DG.IsConnected(g, n, m);
+            reveal DG.PathValid();
+            forall p: DG.Path<HPNP> | DG.PathValid(g, p)
+                ensures !DP.PathLoop(p)
+            {
+                if |p.v| > 1 {
+                    assert DG.IsConnected(g, p.v[0], p.v[1]);
+                    assert false;
+                } else {
+                    assert !DP.PathLoop(p);
+                }
+            }
+            assert !exists p: DG.Path<HPNP> :: DG.PathValid(g, p) && DP.PathLoop(p);
+            reveal DP.DigraphLoop();
+            assert !DP.DigraphLoop(g);
+        }
+    }
+
+
+    lemma {:vcs_split_on_every_assert} NodeKindToGraphValid(c: Circuit, nk: CNodeKind, hpn: HPNode)
+        requires CircuitValid(c)
+        requires CNodeKindSomewhatValid(nk)
+        requires HierarchyPathValid(c, hpn.hp)
+        requires !nk.CHier?
+        ensures DG.DigraphValid(NodeKindToGraph(c, nk, hpn))
+    {
+        var g := NodeKindToGraph(c, nk, hpn);
+        //var bound := NodeKindBound(c, nk, hpn.n);
+        //assert g.NodeBound == bound;
+        //NodeKindBoundBinds(c, nk, hpn);
+        //assert forall n: HPNP :: g.IsNode(n) ==> g.NodeMap(n) < bound;
+        //var max_index := HPNPElementBound(c);
+        //assert g.NodeBound == NodeKindBound(c, nk, hpn.n);
+        //assert (forall n: HPNP :: g.NodeMap(n) >= g.NodeBound ==> !g.IsNode(n));
+        if nk.CComb? {
+            CNodeKindNoSelfPaths(nk);
+        }
+        reveal DG.IsConnected();
+        assert (forall n: HPNP :: !DG.IsConnected(g, n, n));
+        assert (forall n: HPNP, m: HPNP :: DG.IsConnected(g, n, m) ==> DG.IsNode(g, n) && DG.IsNode(g, m));
+        //HPNPToNatInjectiveAll();
+        //NatToHPNPInjectiveAll();
+        //forall hpnp: HPNP {
+        //    HPNPToNatToHPNP(hpnp);
+        //}
+        //assert (forall n: HPNP, m: HPNP :: n != m ==> g.NodeMap(n) != g.NodeMap(m));
+        //assert (forall n: HPNP :: g.InvNodeMap(g.NodeMap(n)) == Some(n));
+        //assert Functions.Injective(g.NodeMap) && Functions.Injective(g.InvNodeMap);
+        reveal DG.DigraphValid();
+        assert DG.DigraphValid(g);
+    }
+
+    function NodeKindHPNPs(c: Circuit, nk: CNodeKind, hpn: HPNode): set<HPNP>
+    {
+        {}
+    }
+
+    function NodeKindConnections(c: Circuit, nk: CNodeKind, hpn: HPNode): set<(HPNP, HPNP)>
+    {
+            //(n: HPNP, m: HPNP) =>
+            //    match nk
+            //        case CComb(_, _, path_exists, _, _) =>
+            //            n.hpn == hpn && m.hpn == hpn && path_exists(n.p, m.p)
+            //        case _ => false,
+        {}
+    }
+
+    function NodeKindToGraph(c: Circuit, nk: CNodeKind, hpn: HPNode): (r: DG.Digraph<HPNP>)
+        requires CircuitValid(c)
+        requires !nk.CHier?
+    {
+        DG.Digraph(
+            NodeKindHPNPs(c, nk, hpn),
+            NodeKindConnections(c, nk, hpn)
+        )
+    }
+
+    function NewNode(c: Circuit): CNode
+    {
+        0
+    }
+
+    lemma AddNodeNoInputsAddDGNode(c: Circuit, nk: CNodeKind)
+        // This is equivalent to adding many nodes to the digraph.
+        // One node for each port (if it's not hierarchical)
+
+        // Assume it's not Hierarchical.
+        // Show that the CNode creates a subgraph.
+        // Show that the subgraph contains no loops.
+        // Show that the combining the subgraphs does not
+        // introduce loops.
+        requires CNodeKindSomewhatValid(nk)
+        requires CircuitValid(c)
+        requires CircuitNoLoops(c)
+        requires !nk.CHier?
+        ensures
+            var (new_c, n) := AddNodeNoInputs(c, nk);
+            var g := CtoG(c);
+            var new_g := CtoG(new_c);
+            DG.DigraphValid(g) &&
+            !DP.DigraphLoop(g) &&
+            true
+            //DG.DigraphValid(new_g) &&
+            //!DP.DigraphLoop(new_g)
+    {
+        var new_node := NewNode(c);
+        var g := CtoG(c);
+        assert !DP.DigraphLoop(g);
+        var hpn := HPNode(HP([]), new_node);
+        var sg := NodeKindToGraph(c, nk, hpn);
+        reveal CircuitValid();
+        assert CircuitNodeKindValid(c);
+        NodeKindToGraphValid(c, nk, hpn);
+        NodeKindToGraphNoLoop(c, nk, hpn);
+        assert DG.DigraphValid(sg);
+        assert !DP.DigraphLoop(sg);
+        HPNodeNotInCircuitHPNPNotInGraph(c, hpn);
+        reveal DC.DigraphsCompatible();
+        reveal CtoG();
+        assert DC.DigraphsCompatible(g, sg);
+        CtoGValid(c);
+        var new_g := DC.Combine(g, sg);
+        DC.CombineValid(g, sg);
+        DC.CombineNoLoops(g, sg);
+        assert DG.DigraphValid(new_g);
+        assert !DP.DigraphLoop(new_g);
+
+        var (new_c, n) := AddNodeNoInputs(c, nk);
+        var new_g2 := CtoG(new_c);
+    }
 
     function AddNodeNoInputs(c: Circuit, nk: CNodeKind): (r: (Circuit, CNode))
         requires CircuitValid(c)
@@ -223,25 +436,22 @@ module CircuitBuild {
         ensures CircuitValid(r.0)
     {
         reveal CircuitValid();
-        var new_node := c.NodeBound;
-        var nk_port_bound := NKPortBound(nk);
+        var new_node := NewNode(c);
         var new_c := Circuit(
-            NodeKind := n => if n == new_node then Some(nk) else c.NodeKind(n),
+            NodeKind := c.NodeKind[new_node := nk],
             PortSource := c.PortSource,
-            NodeBound := c.NodeBound+1,
-            PortBound := if nk_port_bound > c.PortBound then nk_port_bound else c.PortBound,
+            //NodeBound := c.NodeBound+1,
+            //PortBound := if nk_port_bound > c.PortBound then nk_port_bound else c.PortBound,
             HierLevel := c.HierLevel,
             PortNames := c.PortNames
         );
-        assert new_node < new_c.NodeBound;
-        assert forall n: CNode :: (new_c.NodeKind(n) == (if (n == new_node) then
-            Some(nk) else c.NodeKind(n))) ;
+        assert forall n: CNode :: (NodeKind(new_c, n) == (if (n == new_node) then
+            Some(nk) else NodeKind(c, n))) ;
         assert CircuitNodeKindValid(c);
-        assert CircuitPortSourceValid(c);
-        assert forall p: CPort ::
-                (IsIPort(nk, p) ==> p < new_c.PortBound) &&
-                (IsOPort(nk, p) ==> p < new_c.PortBound);
-        assert CNodeKindValid(new_c.HierLevel, new_c.PortBound, nk);
+        assert CircuitNodeKindValid(new_c);
+        assert CircuitPortSourceValid(new_c);
+        assert CircuitValid(new_c);
+        assert CNodeKindValid(new_c.HierLevel, nk);
         (new_c, new_node)
     }
 
@@ -251,25 +461,26 @@ module CircuitBuild {
         ensures CircuitValid(r.0)
     {
         reveal CircuitValid();
-        var new_node := c.NodeBound;
+        var new_node := NewNode(c);
         var new_c := Circuit(
-            NodeKind := n => if n == new_node then Some(nk) else c.NodeKind(n),
-            PortSource := (inp: NP) =>
-                if inp.n == new_node then
-                    if inp.p in ip then
-                        Some(ip[inp.p])
-                    else
-                        None
-                else
-                    c.PortSource(inp),
-            NodeBound := c.NodeBound+1,
-            PortBound := c.PortBound,
+            NodeKind := c.NodeKind[new_node := nk],
+            PortSource := c.PortSource, // FIXME: Should update
+            //NodeKind := n => if n == new_node then Some(nk) else c.NodeKind(n),
+            //PortSource := (inp: NP) =>
+            //    if inp.n == new_node then
+            //        if inp.p in ip then
+            //            Some(ip[inp.p])
+            //        else
+            //            None
+            //    else
+            //        c.PortSource(inp),
+            //NodeBound := c.NodeBound+1,
+            //PortBound := c.PortBound,
             HierLevel := c.HierLevel,
             PortNames := c.PortNames
         );
-        assert new_node < new_c.NodeBound;
-        assert forall n: CNode :: (new_c.NodeKind(n) == (if (n == new_node) then
-            Some(nk) else c.NodeKind(n))) ;
+        assert forall n: CNode :: (NodeKind(new_c, n) == (if (n == new_node) then
+            Some(nk) else NodeKind(c, n))) ;
         assert CircuitNodeKindValid(c);
         assert CircuitPortSourceValid(c);
         (c, new_node)
