Test/Primitives.dfy
@@ -2,7 +2,6 @@ module Primitives {
 
     import opened Std.Wrappers
     import C = CircuitBase
-    import opened CircuitValidity
 
     function XorBehav(m: map<C.CPort, bool>): Option<map<C.CPort, bool>>
     {
@@ -37,7 +36,7 @@ module Primitives {
     const xor_port_bound: C.CPort := 3
 
     lemma nk_xor_valid()
-        ensures CNodeKindValid(0, xor_port_bound, nk_xor)
+        ensures C.CNodeKindValid(0, xor_port_bound, nk_xor)
     {
     }
 
